Update clos_to_bvlProof for #244 and #245

compiler/backend/semantics/bvlSemScript.sml
@@ -82,8 +82,10 @@ val _ = export_rewrites["do_eq_def"];
 val _ = Parse.temp_overload_on("Error",``(Rerr(Rabort Rtype_error)):(bvlSem$v#'ffi bvlSem$state,bvlSem$v)result``)
 
 (* same as closSem$do_app, except:
-    - LengthByteVec and DerefByteVec are removed
+    - LengthByteVec, DerefByteVec, and ConcatByteVec are removed
     - FromListByte and String produces ByteArrays rather than ByteVectors
+    - ByteVecToArr, ByteVecFromArr simply change the tag on the ByteArray
+    - ConcatByte respects compare-by-contents tag
     - Label is added *)
 
 val do_app_def = Define `
@@ -144,6 +146,19 @@ val do_app_def = Define `
                  (ptr, ByteArray f (LUPDATE (i2w b) (Num i) bs)))
              else Error)
          | _ => Error)
+    | (ConcatByte fl,[lv]) =>
+        (case v_to_list lv of
+         | SOME vs =>
+           (case
+              (some wss. ∃ps.
+                v_to_list lv = SOME (MAP RefPtr ps) ∧
+                MAP (FLOOKUP s.refs) ps = MAP (SOME o ByteArray fl) wss)
+            of SOME wss =>
+              let ptr = (LEAST ptr. ¬(ptr IN FDOM s.refs)) in
+                Rval (RefPtr ptr, s with refs := s.refs |+
+                         (ptr,ByteArray fl (FLAT wss)))
+            | _ => Error)
+         | _ => Error)
     | (FromList n,[lv]) =>
         (case v_to_list lv of
          | SOME vs => Rval (Block n vs, s)
@@ -158,6 +173,20 @@ val do_app_def = Define `
                          Rval (RefPtr ptr, s with refs := s.refs |+
                            (ptr,ByteArray T (MAP n2w ns)))
           | NONE => Error)
+    | (ByteVecToArr,[RefPtr ptr]) =>
+        (case FLOOKUP s.refs ptr of
+         | SOME (ByteArray T ws) =>
+             let ptr = (LEAST ptr. ¬(ptr IN FDOM s.refs)) in
+               Rval (RefPtr ptr, s with refs := s.refs |+
+                     (ptr, ByteArray F ws))
+         | _ => Error)
+    | (ByteVecFromArr,[RefPtr ptr]) =>
+        (case FLOOKUP s.refs ptr of
+         | SOME (ByteArray F ws) =>
+             let ptr = (LEAST ptr. ¬(ptr IN FDOM s.refs)) in
+               Rval (RefPtr ptr, s with refs := s.refs |+
+                     (ptr, ByteArray T ws))
+         | _ => Error)
     | (TagEq n,[Block tag xs]) =>
         Rval (Boolv (tag = n), s)
     | (TagLenEq n l,[Block tag xs]) =>
